erasure/theories/EWcbvEvalEtaInd.v
@@ -1,0 +1,653 @@
+(* Distributed under the terms of the MIT license. *)
+From Coq Require Import Utf8 Program ssreflect ssrbool.
+From MetaCoq.Template Require Import config utils Kernames BasicAst EnvMap.
+From MetaCoq.Erasure Require Import EAst EAstUtils EInduction EWcbvEval EGlobalEnv ECSubst EInduction EWcbvEvalInd EEtaExpanded.
+
+Set Asymmetric Patterns.
+From Equations Require Import Equations.
+Set Equations Transparent.
+Local Set Keyed Unification.
+
+#[export]
+Hint Constructors eval : core.
+
+Definition atomic_term (t : term) :=
+  match t with
+  | tBox | tConstruct _ _ | tConst _ | tRel _ | tVar _ => true
+  | _ => false
+  end.
+
+Section OnSubterm.
+
+  Inductive on_subterms (Q : nat -> term -> Type) (n : nat) : term -> Type :=
+  | on_atom t : atomic_term t -> on_subterms Q n t
+  | on_evar k l : All (Q n) l -> on_subterms Q n (tEvar k l)
+  | on_lambda na t : Q (S n) t -> on_subterms Q n (tLambda na t)
+  | on_letin na t u : Q n t -> Q (S n) u -> on_subterms Q n (tLetIn na t u)
+  | on_app f u : Q n f -> Q n u -> on_subterms Q n (tApp f u)
+  | on_case ci discr brs : Q n discr -> 
+    All (fun br => Q (#|br.1| + n) br.2) brs -> on_subterms Q n (tCase ci discr brs)
+  | on_proj p c : Q n c -> on_subterms Q n (tProj p c)
+  | on_fix mfix idx : All (fun d => Q (#|mfix| + n) d.(dbody)) mfix -> on_subterms Q n (tFix mfix idx)
+  | on_cofix mfix idx : All (fun d => Q (#|mfix| + n) d.(dbody)) mfix -> on_subterms Q n (tCoFix mfix idx).
+  Derive Signature for on_subterms.
+End OnSubterm.
+
+Class Qdummy (Q : nat -> term -> Type) := qdummy : forall n, Q n tDummy.
+#[export] Hint Mode Qdummy ! : typeclass_instances.
+
+Class Qpres (Q : nat -> term -> Type) := qpres : forall n t, Q n t -> on_subterms Q n t.
+#[export] Hint Mode Qpres ! : typeclass_instances.
+Class Qapp (Q : nat -> term -> Type) := qapp : forall n f args, Q n (mkApps f args) <~> Q n f × All (Q n) args.
+#[export] Hint Mode Qapp ! : typeclass_instances.
+Class Qcase (Q : nat -> term -> Type) := qcase : forall n ci discr brs, Q n (tCase ci discr brs) <~> Q n discr × All (fun br => Q (#|br.1| + n) br.2) brs.
+#[export] Hint Mode Qcase ! : typeclass_instances.
+Class Qproj (Q : nat -> term -> Type) := qproj : forall n p discr, Q n (tProj p discr) <~> Q n discr.
+#[export] Hint Mode Qproj ! : typeclass_instances.
+Class Qfix (Q : nat -> term -> Type) := qfix : forall n mfix idx, Q n (tFix mfix idx) <~>  All (fun d => Q (#|mfix| + n) d.(dbody)) mfix.
+#[export] Hint Mode Qfix ! : typeclass_instances.
+Class Qcofix (Q : nat -> term -> Type) := qcofix : forall n mfix idx, Q n (tCoFix mfix idx) <~>  All (fun d => Q (#|mfix| + n) d.(dbody)) mfix.
+#[export] Hint Mode Qcofix ! : typeclass_instances.
+Class Qsubst (Q : nat -> term -> Type) := qsubst : forall t l, Q (#|l|) t -> All (Q 0) l -> Q 0 (substl l t).
+#[export] Hint Mode Qsubst ! : typeclass_instances.
+Class Qfixs (Q : nat -> term -> Type) := qfixs : forall mfix idx, Q 0 (tFix mfix idx) -> 
+    forall args fn, cunfold_fix mfix idx = Some (args, fn) ->
+    Q 0 fn.
+#[export] Hint Mode Qfixs ! : typeclass_instances.
+Class Qcofixs (Q : nat -> term -> Type) := qcofixs : forall mfix idx, Q 0 (tCoFix mfix idx) -> 
+  forall args fn, cunfold_cofix mfix idx = Some (args, fn) ->
+  Q 0 fn.
+#[export] Hint Mode Qcofixs ! : typeclass_instances.
+      
+Lemma Qfix_subst mfix Q : Qfix Q -> All (λ d : def term, Q (#|mfix| + 0) (dbody d)) mfix -> All (Q 0) (fix_subst mfix).
+Proof.
+  intros qfix; unfold fix_subst.
+  generalize #|mfix| at 2. intros n hfix.
+  induction n; constructor; auto.
+  now eapply qfix.
+Qed.
+
+Lemma Qcofix_subst mfix Q : Qcofix Q -> All (λ d : def term, Q (#|mfix| + 0) (dbody d)) mfix -> All (Q 0) (cofix_subst mfix).
+Proof.
+  intros qfix; unfold cofix_subst.
+  generalize #|mfix| at 2. intros n hfix.
+  induction n; constructor; auto.
+  now eapply qfix.
+Qed.
+
+#[export] Instance Qsubst_Qfixs Q : Qpres Q -> Qfix Q -> Qsubst Q -> Qfixs Q.
+Proof.
+  move=> qpres qfix; rewrite /Qsubst /Qfixs.
+  intros Hs mfix idx hfix args fn.
+  rewrite /cunfold_fix.
+  eapply qpres in hfix. depelim hfix => //.
+  destruct nth_error eqn:hnth => //.
+  eapply nth_error_all in hnth; tea. cbn in hnth.
+  rewrite Nat.add_0_r in hnth.
+  intros [= <-]. subst fn.
+  eapply Hs. rewrite fix_subst_length //.
+  now apply Qfix_subst.
+Qed.
+
+#[export] Instance Qsubst_Qcofixs Q : Qpres Q -> Qcofix Q -> Qsubst Q -> Qcofixs Q.
+Proof.
+  move=> qpres qfix; rewrite /Qsubst /Qcofixs.
+  intros Hs mfix idx hfix args fn.
+  rewrite /cunfold_cofix.
+  eapply qpres in hfix. depelim hfix => //.
+  destruct nth_error eqn:hnth => //.
+  eapply nth_error_all in hnth; tea. cbn in hnth.
+  rewrite Nat.add_0_r in hnth.
+  intros [= <-]. subst fn.
+  eapply Hs. rewrite cofix_subst_length //.
+  now apply Qcofix_subst.
+Qed.
+
+Class Qconst Σ (Q : nat -> term -> Type) := qconst :
+  ∀ kn decl, declared_constant Σ kn decl → 
+    match cst_body decl with
+    | None => unit
+    | Some b => Q 0 b
+    end.
+#[export] Hint Mode Qconst - ! : typeclass_instances.
+
+Definition isConstructApp c := isConstruct (decompose_app c).1.
+
+Class Qpreserves (Q : nat -> term -> Type) Σ :=
+  { qpres_qpres :> Qpres Q;
+    qpres_qcons :> Qconst Σ Q;
+    qpres_qapp :> Qapp Q;
+    qpres_qcase :> Qcase Q;
+    qpres_qproj :> Qproj Q;
+    qpres_qsubst :> Qsubst Q;
+    qpres_qfix :> Qfix Q;
+    qpres_qcofix :> Qcofix Q;
+    qpres_qdummy :> Qdummy Q }.
+
+Lemma eval_preserve_mkApps_ind :
+∀ (wfl : WcbvFlags) (Σ : global_declarations) 
+  (P' : term → term → Type)
+  (Q : nat -> term -> Type)
+  {Qpres : Qpreserves Q Σ}
+  (P := (fun x y => [× P' x y, Q 0 x, Q 0 y, isEtaExp Σ x & isEtaExp Σ y])%type)
+  (HPQ : ∀ t u, eval Σ t u -> Q 0 t -> P' t u -> Q 0 u),
+  isEtaExp_env Σ ->
+  wf_glob Σ ->
+  (∀ (a t t' : term),
+	 eval Σ a tBox ->
+     P a tBox →
+     eval Σ t t' → P t t' → P' (tApp a t) tBox) → 
+  (∀ (f0 : term) (na : name) (b a a' res : term),
+      eval Σ f0 (tLambda na b) → 
+      P f0 (tLambda na b)
+         → eval Σ a a'
+           → P a a'
+             → eval Σ (ECSubst.csubst a' 0 b) res
+          → P (ECSubst.csubst a' 0 b) res → P' (tApp f0 a) res)
+    → (∀ (na : name) (b0 b0' b1 res : term),
+         eval Σ b0 b0'
+         → P b0 b0'
+         -> isEtaExp Σ b1
+           → eval Σ (ECSubst.csubst b0' 0 b1) res
+             → P (ECSubst.csubst b0' 0 b1) res → 
+             P' (tLetIn na b0 b1) res)
+      → (∀ (ind : inductive) (pars : nat) (discr : term) 
+           (c : nat) (args : list term) (brs : 
+                                              list 
+                                                (list name × term)) 
+           (br : list name × term) (res : term),
+           forallb (λ x : list name × term, isEtaExp Σ x.2) brs ->
+           eval Σ discr (mkApps (tConstruct ind c) args)
+           → P discr (mkApps (tConstruct ind c) args)
+             → inductive_isprop_and_pars Σ ind = Some (false, pars)
+               → nth_error brs c = Some br
+                 → #|skipn pars args| = #|br.1|
+                   → eval Σ (iota_red pars args br) res
+                     → P (iota_red pars args br) res
+                       → P' (tCase (ind, pars) discr brs) res)
+        → (∀ (ind : inductive) (pars : nat) (discr : term) 
+             (brs : list (list name × term)) 
+             (n : list name) (f3 res : term),
+             with_prop_case
+             → eval Σ discr tBox
+               → P discr tBox
+                 → inductive_isprop_and_pars Σ ind = Some (true, pars)
+                   → brs = [(n, f3)]
+                   -> forallb (isEtaExp Σ ∘ snd) brs
+                     → eval Σ (ECSubst.substl (repeat tBox #|n|) f3)
+                         res
+                       → P (ECSubst.substl (repeat tBox #|n|) f3) res
+                         → P' (tCase (ind, pars) discr brs) res)
+          → (∀ (f4 : term) (mfix : mfixpoint term) 
+               (idx : nat) (argsv : list term) 
+               (a av fn res : term),
+               with_guarded_fix ->
+               eval Σ f4 (mkApps (tFix mfix idx) argsv)
+               → P f4 (mkApps (tFix mfix idx) argsv)
+                 → eval Σ a av
+                   → P a av
+                     → cunfold_fix mfix idx = Some (#|argsv|, fn)
+                     -> isEtaExp Σ fn
+                      → eval Σ (tApp (mkApps fn argsv) av) res
+                         → P (tApp (mkApps fn argsv) av) res
+                           → P' (tApp f4 a) res)
+            → (∀ (f5 : term) (mfix : mfixpoint term) 
+                 (idx : nat) (argsv : list term) 
+                 (a av : term) (narg : nat) (fn : term),
+                 with_guarded_fix ->
+                 eval Σ f5 (mkApps (tFix mfix idx) argsv)
+                 → P f5 (mkApps (tFix mfix idx) argsv)
+                   → eval Σ a av
+                     → P a av
+                       → cunfold_fix mfix idx = Some (narg, fn)
+                         → #|argsv| < narg
+                         -> isEtaExp Σ (tApp (mkApps (tFix mfix idx) argsv) av)
+                           → P' (tApp f5 a)
+                               (tApp
+                                  (mkApps (tFix mfix idx) argsv) av))
+            → (∀ (f5 : term) (mfix : mfixpoint term) 
+            (idx : nat) (a av : term) (narg : nat) (fn : term) res,
+            with_guarded_fix = false ->
+            eval Σ f5 (tFix mfix idx)
+            → P f5 (tFix mfix idx)
+              → cunfold_fix mfix idx = Some (narg, fn)
+              -> isEtaExp Σ fn
+              -> isEtaExp Σ a
+              → eval Σ (tApp fn a) res   
+              → P (tApp fn a) res
+              -> isEtaExp Σ (tApp f5 a)
+              → P' (tApp f5 a) res) → 
+              
+              (∀ (ip : inductive × nat) (mfix : mfixpoint term) 
+                   (idx : nat) (args : list term) 
+                   (narg : nat) discr (fn : term) (brs : 
+                                                 list 
+                                                 (list name × term)) 
+                   (res : term),
+                   cunfold_cofix mfix idx = Some (narg, fn)
+                   -> isEtaExp Σ fn
+                   -> forallb (isEtaExp Σ) args
+                   -> eval Σ discr (mkApps (tCoFix mfix idx) args)
+                   -> P discr (mkApps (tCoFix mfix idx) args)
+                   -> forallb (isEtaExp Σ ∘ snd) brs
+                   → eval Σ (tCase ip (mkApps fn args) brs) res
+                     → P (tCase ip (mkApps fn args) brs) res
+                       → P'
+                           (tCase ip discr brs)
+                           res)
+                → (∀ (p : projection) (mfix : mfixpoint term) 
+                     (idx : nat) (args : list term) 
+                     (narg : nat) discr (fn res : term),
+                     cunfold_cofix mfix idx = Some (narg, fn)
+                     -> isEtaExp Σ fn
+                     -> forallb (isEtaExp Σ) args
+                     -> eval Σ discr (mkApps (tCoFix mfix idx) args)
+                     -> P discr (mkApps (tCoFix mfix idx) args)
+                     → eval Σ (tProj p (mkApps fn args)) res
+                       → P (tProj p (mkApps fn args)) res
+                         → P'
+                             (tProj p discr) res)
+                  → (∀ (c : kername) (decl : constant_body) 
+                       (body : term),
+                       declared_constant Σ c decl
+                       → ∀ res : term,
+                           cst_body decl = Some body
+                           → eval Σ body res
+                             → P body res → P' (tConst c) res)
+                    → (∀ (i : inductive) (pars arg : nat) 
+                         (discr : term) (args : list term) 
+                         (res : term),
+                         eval Σ discr
+                           (mkApps (tConstruct i 0) args)
+                         → P discr (mkApps (tConstruct i 0) args)
+                           → inductive_isprop_and_pars Σ i = Some (false, pars)
+                             → eval Σ (nth (pars + arg) args tDummy) res
+                               → P (nth (pars + arg) args tDummy) res
+                                 → P' (tProj (i, pars, arg) discr) res)
+                      → (∀ (i : inductive) (pars arg : nat) 
+                           (discr : term),
+                           with_prop_case
+                           → eval Σ discr tBox
+                             → P discr tBox
+                               → inductive_isprop_and_pars Σ i = Some (true, pars)
+                                 → P' (tProj (i, pars, arg) discr)
+                                     tBox) →
+  (∀ (f11 f' : term) a a',
+     forall (ev : eval Σ f11 f'), P f11 f' ->  
+     (forall t u (ev' : eval Σ t u), eval_depth ev' <= eval_depth ev -> Q 0 t -> isEtaExp Σ t -> P t u) →
+     ~~ isConstructApp f11 ->
+     ~~ (isLambda f' || (if with_guarded_fix then isFixApp f' else isFix f') || isBox f') → 
+     eval Σ a a' → P a a' → 
+     isEtaExp Σ (tApp f' a') ->
+     P' (tApp f11 a) (tApp f' a')) → 
+  (∀ ind i args args',
+    All2 (eval Σ) args args' -> 
+    isEtaExp_app Σ ind i #|args| ->
+    Q 0 (mkApps (tConstruct ind i) args) -> Q 0 (mkApps (tConstruct ind i) args') ->
+    All2 P args args' ->
+    P' (mkApps (tConstruct ind i) args) (mkApps (tConstruct ind i) args')) → 
+  (∀ t : term, atom t → Q 0 t -> isEtaExp Σ t -> P' t t) ->
+  ∀ (t t0 : term), Q 0 t -> isEtaExp Σ t -> eval Σ t t0 → P' t t0.
+Proof.
+  intros * Qpres P P'Q etaΣ wfΣ.
+  assert (qfixs: Qfixs Q) by tc.
+  assert (qcofixs: Qcofixs Q) by tc.
+  intros.
+  enough (P' t t0 × isEtaExp Σ t0). apply X16.
+  pose proof (p := @Fix_F { t : _ & { t0 : _ & { qt : Q 0 t & eval Σ t t0 }}}).
+  specialize (p (MR lt (fun x => eval_depth x.π2.π2.π2))).
+  set(foo := existT _ t (existT _ t0 (existT _ X15 H0)) :  { t : _ & { t0 : _ & { qt : Q 0 t & eval Σ t t0 }}}).
+  move: H.
+  change t with (projT1 foo).
+  change t0 with (projT1 (projT2 foo)).
+  change H0 with (projT2 (projT2 foo)).
+  revert foo.
+  match goal with
+    |- let foo := _ in @?P foo => specialize (p (fun x => P x))
+  end.
+  forward p.
+  2:{ apply p. apply measure_wf, lt_wf. }
+  clear p.
+  rename X15 into qt.
+  clear t t0 qt H0.
+  intros (t & t0 & qt & ev). 
+  intros IH.
+  set (IH' t t0 q H := IH (t; t0; q; H)). clearbody IH'; clear IH; rename IH' into IH.
+  Opaque isEtaExp.
+  cbn in IH. unfold MR in IH; cbn in IH. cbn.
+  Ltac ih := 
+    match goal with 
+    [ IH : forall x y, ?Q 0 x -> _ |- _ ] => unshelve eapply IH; tea; cbn; try lia
+    end.
+  Ltac iheta e := 
+    match goal with 
+    [ IH : forall x y, ?Q 0 x -> _ |- _ ] => unshelve eapply (IH _ _ e); tea; cbn; try lia
+    end.
+  Ltac hp' P'Q := intros [hp' heta]; repeat split => //; try eapply P'Q; tea.
+  assert (and_assum : forall x y, (P' x y × isEtaExp Σ y) -> 
+    ((P' x y × isEtaExp Σ y) -> Q 0 x × Q 0 y × isEtaExp Σ x) ->
+    P x y).    
+  { intuition auto. red. intuition auto. }
+  Ltac ih' P'Q :=
+    match goal with
+    | [ H : _, IH : forall x y, ?Q 0 x -> _ |- _ ] =>
+      eapply H; tea; (apply and_assum; [ih|hp' P'Q])
+    end.
+  destruct ev.
+  1-14:eapply qpres in qt; depelim qt => //.  
+  all:try solve [ih' P'Q].
+  - move/isEtaExp_tApp.
+    destruct decompose_app as [hd args] eqn:da.
+    destruct (construct_viewc hd) eqn:cv.
+    * move=> [] argsn [] ha [] ht /andP[] etaind etaargs.
+      clear IH; rewrite ha in ev1. elimtype False.
+      eapply eval_construct in ev1 as [ex []]. solve_discr.
+    * move=> /and4P [] etat0 etaargs etaa etat.
+      split. eapply X; tea; (apply and_assum; [ih|hp' P'Q]).
+      iheta q.
+  - move/isEtaExp_tApp.
+    destruct decompose_app as [hd args] eqn:da.
+    destruct (construct_viewc hd) eqn:cv.
+    * move=> [] argsn [] ha [] ht /andP[] etaind etaargs.
+      clear IH; rewrite ha in ev1. elimtype False.
+      eapply eval_construct in ev1 as [ex []]. solve_discr.
+    * move=> /and4P [] etat0 etaargs etaa etat. 
+      assert (ql : Q 0 (tLambda na b)).
+      { eapply P'Q; tea. ih. }
+       assert (qs: Q 0 (csubst a' 0 b)).
+      { eapply qpres in ql. depelim ql => //.
+        eapply (qsubst b [a']) in q1. now cbn in q1.
+        repeat constructor.
+        eapply P'Q; tea; ih. }
+      assert (isEtaExp Σ (csubst a' 0 b)).
+      { eapply etaExp_csubst; tea. cbn in IH. specialize (IH _ _ q0 ev2). apply IH; [lia|auto].
+        specialize (IH _ _ q ev1). forward IH by cbn; lia.
+        forward IH by auto. destruct IH as [_ eta]. now simp_eta in eta. }
+      split. eapply X0; tea. 1-3:(apply and_assum; [ih|hp' P'Q]).
+      iheta qs.
+  - simp_eta. move=> /andP[etab0 etab1].
+    assert (qs : Q 0 (csubst b0' 0 b1)).
+    { eapply (qsubst b1 [b0']) in q0. now cbn in q0.
+      repeat constructor.
+      eapply P'Q; tea; ih. }
+    assert (isEtaExp Σ (csubst b0' 0 b1)).
+    { eapply etaExp_csubst; tea. iheta q. }
+    split; [eapply X1; tea|]. 1-2:(apply and_assum; [ih|hp' P'Q]).
+    iheta qs.
+  - simp_eta. move=> /andP[etad etabrs].
+    assert (isEtaExp Σ (iota_red pars args br)).
+    { eapply isEtaExp_iota_red.
+      assert (isEtaExp Σ (mkApps (tConstruct ind c) args)) by iheta q.
+      rewrite isEtaExp_mkApps_napp /= // in H.
+      now move/andP: H => [].
+      now clear IH; eapply nth_error_forallb in e0; tea. }
+    assert (Q 0 (iota_red pars args br)).
+    { unfold iota_red.
+      eapply nth_error_all in a; tea. cbn in a.
+      rewrite -e1 in a.
+      rewrite -(List.rev_length (skipn pars args)) in a.
+      rewrite Nat.add_0_r in a.
+      eapply (qsubst _ (List.rev (skipn pars args))) in a.
+      2:{ eapply All_rev, All_skipn. 
+        assert (Q 0 (mkApps (tConstruct ind c) args)).
+        eapply P'Q; tea; ih.
+        eapply qapp in X15; tea. eapply X15. }
+      exact a. }
+    split. eapply X2; tea. 1-2:(apply and_assum; [ih|hp' P'Q]).
+    iheta X15.
+  - simp_eta; move=> /andP[etad etabrs].
+    assert (isEtaExp Σ (substl (repeat tBox #|n|) f)).
+    { eapply isEtaExp_substl => //. rewrite forallb_repeat //.
+      rewrite e0 /= in etabrs. now move/andP: etabrs. }
+    assert (Q 0 (substl (repeat tBox #|n|) f)).
+    { subst brs. eapply All_tip in a. cbn in a.
+      rewrite -(repeat_length tBox #|n|) Nat.add_0_r in a.
+      eapply (qsubst _ (repeat tBox #|n|)) in a => //.
+      eapply All_repeat. eapply P'Q; tea; ih. }
+   split. eapply X3; tea; (apply and_assum; [ih|hp' P'Q]).
+   iheta X15.
+  - move/isEtaExp_tApp.
+    destruct decompose_app as [hd args] eqn:da.
+    destruct (construct_viewc hd) eqn:cv.
+    * move=> [] argsn [] ha [] ht /andP[] etaind etaargs.
+      clear IH; rewrite ha in ev1. elimtype False.
+      eapply eval_construct in ev1 as [ex []]. solve_discr.
+    * move=> /and4P [] etat0 etaargs etaa etat. 
+      assert (qa : Q 0 (tApp (mkApps fn argsv) av)).
+      { pose proof (ev1' := ev1). eapply P'Q in ev1' => //.
+        eapply qapp in ev1' as [hfix qargs] => //.
+        rewrite -[tApp _ _](mkApps_app _ _ [av]).
+        eapply (qapp _ _ _).2.
+        split => //.
+        eapply (qfixs mfix idx) in hfix; tea.
+        eapply All_app_inv => //. eapply All_tip.1.
+        eapply P'Q; tea; ih. clear ev1'; ih. }
+      assert (etaapp : isEtaExp Σ fn × isEtaExp Σ (tApp (mkApps fn argsv) av)).
+      { rewrite -[tApp _ _](mkApps_app _ _ [av]).
+        assert (hfix : isEtaExp Σ (mkApps (tFix mfix idx) argsv)) by iheta q.
+        rewrite isEtaExp_mkApps_napp /= // in hfix.
+        move/andP: hfix => [hfix hargs].
+        apply EWcbvEvalInd.and_assum.
+        eapply isEtaExp_cunfold_fix. now simp_eta in hfix. exact e.
+        intros hfn.
+        eapply isEtaExp_mkApps_intro => //.        
+        eapply All_app_inv. now eapply forallb_All in hargs. eapply (fst All_tip).
+        iheta q0. }
+      destruct etaapp as [etafn etafnapp].
+      split. eapply X4; tea; (apply and_assum; [ih|hp' P'Q]).
+      iheta qa.
+  - move/isEtaExp_tApp.
+    destruct decompose_app as [hd args] eqn:da.
+    destruct (construct_viewc hd) eqn:cv.
+    * move=> [] argsn [] ha [] ht /andP[] etaind etaargs.
+      clear IH; rewrite ha in ev1. elimtype False.
+      eapply eval_construct in ev1 as [ex []]. solve_discr.
+    * move=> /and4P [] etat0 etaargs etaa etat.
+      assert (isEtaExp Σ (tApp (mkApps (tFix mfix idx) argsv) av)).
+      { rewrite -[tApp _ _](mkApps_app _ _ [av]).
+        rewrite isEtaExp_mkApps_napp // /=.
+        assert (isEtaExp Σ (mkApps (tFix mfix idx) argsv)) by iheta q.
+        assert (isEtaExp Σ av) by iheta q0.
+        rewrite isEtaExp_mkApps_napp // /= in H.
+        move/andP: H => [] -> /=.
+        rewrite forallb_app /= H0 => -> /= //. }
+      split => //. eapply X5; tea; (apply and_assum; [ih|hp' P'Q]).
+  - move/isEtaExp_tApp.
+    destruct decompose_app as [hd args] eqn:da.
+    destruct (construct_viewc hd) eqn:cv.
+    * move=> [] argsn [] ha [] ht /andP[] etaind etaargs.
+      clear IH; rewrite ha in ev1. elimtype False.
+      eapply eval_construct in ev1 as [ex []]. solve_discr.
+    * move=> /and4P [] etat0 etaargs etaa etat. 
+      assert (qa : Q 0 (tApp fn a)).
+      { pose proof (ev1' := ev1). eapply P'Q in ev1' => //. 2:clear ev1'; ih.
+        eapply qfixs in ev1'. cbn in IH. eapply ev1' in e.
+        eapply (qapp _ _ [a]); split => //. now eapply All_tip.1. }
+      assert (etafn : isEtaExp Σ fn).
+      { assert (hfix : isEtaExp Σ (tFix mfix idx)) by iheta q.
+        eapply isEtaExp_cunfold_fix. now simp_eta in hfix. exact e. }
+      assert (etaapp : isEtaExp Σ (tApp fn a)).
+      { change (isEtaExp Σ (mkApps fn [a])).
+        eapply isEtaExp_mkApps_intro => //.
+        now eapply All_tip.1. }
+      split. eapply X6; tea. 1-2:(apply and_assum; [ih|hp' P'Q]).
+      rewrite (decompose_app_inv da). eapply isEtaExp_mkApps_intro => //.
+      now eapply forallb_All in etaargs.
+      iheta qa.
+  - simp_eta. move=> /andP[etad etabrs].
+    assert (qa : Q 0 (tCase ip (mkApps fn args) brs)).
+    { pose proof (ev1' := ev1). eapply P'Q in ev1' => //.
+      eapply qapp in ev1' as [hfix qargs] => //.
+      eapply (qcase _ _ _ _).2. split => //.
+      eapply qapp; split => //.
+      eapply (qcofixs mfix idx) in hfix; tea. 
+      clear ev1'; ih. }
+    assert (etafn : isEtaExp Σ fn && forallb (isEtaExp Σ) args).
+    { assert (hfix : isEtaExp Σ (mkApps (tCoFix mfix idx) args)) by iheta q.
+      rewrite isEtaExp_mkApps_napp /= // in hfix.
+      move/andP: hfix => [hfix hargs].
+      apply/andP; split => //.
+      eapply isEtaExp_cunfold_cofix. now simp_eta in hfix. exact e. }
+    move/andP: etafn => [] etaf etaargs.
+    assert (etac : isEtaExp Σ (tCase ip (mkApps fn args) brs)).
+    { simp_eta. rewrite etabrs andb_true_r.
+      eapply isEtaExp_mkApps_intro => //.
+      now eapply forallb_All in etaargs. }
+    split. eapply X7; tea; (apply and_assum; [ih|hp' P'Q]).
+    iheta qa.
+  - simp_eta. move=> etad.
+    cbn in IH.
+    assert (qa : Q 0 (tProj p (mkApps fn args))).
+    { pose proof (ev1' := ev1). eapply P'Q in ev1' => //.
+      eapply qapp in ev1' as [hfix ?].
+      eapply qproj. eapply qapp. split => //.
+      eapply (qcofixs mfix idx) in hfix; tea.
+      clear ev1'; ih. }
+    assert (etafn : isEtaExp Σ fn && forallb (isEtaExp Σ) args).
+    { assert (hfix : isEtaExp Σ (mkApps (tCoFix mfix idx) args)) by iheta q.
+      rewrite isEtaExp_mkApps_napp /= // in hfix.
+      move/andP: hfix => [hfix hargs].
+      apply/andP; split => //.
+      eapply isEtaExp_cunfold_cofix. now simp_eta in hfix. exact e. }
+    move/andP: etafn => [] etaf etaargs.
+    assert (etaa : isEtaExp Σ (tProj p (mkApps fn args))).
+    { simp_eta.
+      eapply isEtaExp_mkApps_intro => //.
+      now eapply forallb_All in etaargs. }
+    split. eapply X8; tea; (apply and_assum; [ih|hp' P'Q]).
+    iheta qa.
+  - move => _.
+    assert (Q 0 body).
+    { cbn in IH; eapply (qconst (Q:=Q)) in isdecl. now rewrite e in isdecl. }
+    assert (isEtaExp Σ body).
+    { eapply isEtaExp_lookup in etaΣ as etad; tea.
+      unfold isEtaExp_decl, isEtaExp_constant_decl in etad.
+      now rewrite e /= in etad. }
+    split. eapply X9; tea; (apply and_assum; [ih|hp' P'Q]).
+    iheta X15.
+  - simp_eta => etadiscr.
+    assert (Q 0 (nth (pars + arg) args tDummy)).
+    { pose proof (ev1' := ev1). eapply P'Q in ev1' => //.
+      eapply qapp in ev1' as [_ qargs].
+      { clear -Qpres qargs. generalize (pars+arg).
+        induction args; cbn.
+        destruct n; apply qdummy.
+        depelim qargs. intros [] => //. now eapply IHargs. }
+      clear ev1'; ih. }
+    assert (isEtaExp Σ (nth (pars + arg) args tDummy)).
+    { assert (isEtaExp Σ (mkApps (tConstruct i 0) args)) by iheta q.
+      move: H; simp_eta.
+      rewrite isEtaExp_mkApps_napp // /=.
+      move=> /andP[] etaapp etaargs.
+      rewrite nth_nth_error. destruct nth_error eqn:hnth.
+      eapply nth_error_forallb in etaargs; tea.
+      unfold tDummy. now simp_eta. }
+    split. eapply X10; tea; (apply and_assum; [ih|hp' P'Q]).
+    iheta X15.
+  - simp_eta => etadiscr.
+    split. unshelve eapply X11; tea; try (intros; apply and_assum; [ih|hp' P'Q]).
+    now idtac.
+  - move/isEtaExp_tApp.
+    destruct decompose_app as [hd args] eqn:da.
+    destruct (construct_viewc hd) eqn:cv.
+    * move=> [] argsn [] ha [] ht /andP[] etaind etaargs.
+      assert (eval_depth ev1 = eval_depth ev1) by reflexivity.
+      set (ev1' := ev1). change ev1 with ev1' in H at 1. clearbody ev1'. move: H.
+      subst f.
+      pose proof (eval_construct_size ev1') as [ex []]. subst f'.
+      cbn in IH. intros eq.
+      assert (All2 (λ x y : term, ∑ ev' : eval Σ x y, eval_depth ev' < S (Nat.max (eval_depth ev1) (eval_depth ev2)))
+        (remove_last args ++ [a]) (ex ++ [a'])).
+      { eapply All2_app. eapply All2_impl; tea; cbn. intros ?? []. exists x0. lia.
+        constructor; [|constructor]. exists ev2. lia. }
+      assert (All (Q 0) (remove_last args ++ [a])).
+      { eapply All_app_inv. eapply qapp in q as []; auto.
+        now eapply All_tip.1. }
+      assert (All (isEtaExp Σ) (remove_last args ++ [a])).
+      { rewrite ht -(remove_last_last args a argsn). now eapply forallb_All. }
+      eapply All2_All_mix_left in X15; tea.
+      assert (All2 (fun x y => P' x y × isEtaExp Σ y) (remove_last args ++ [a]) (ex ++ [a'])).
+      { clear X17. eapply All2_All_mix_left in X15; tea.
+        eapply All2_impl; tea. cbn. intros ? ? [? [? [ev ?]]].
+        eapply (IH _ _ q1 ev). lia. auto. }
+      rewrite (remove_last_last args a argsn) in etaargs.
+      rewrite -[tApp _ _](mkApps_app _ _ [a]).
+      rewrite -[tApp _ _](mkApps_app _ _ [a']).
+      assert (All (fun x => Q 0 x × isEtaExp Σ x) (ex ++ [a'])).
+      { eapply All2_mix in X15; tea. cbn in X15.
+        eapply All2_All_mix_left in X15. 2:exact X16.
+        eapply All2_All_right; tea; cbn.
+        intros ? ? [? [? [? []]]]. split. eapply P'Q; tea. apply p. apply p. }
+      split. 
+      eapply (X13 ind n).
+      + eapply All2_app. eapply All2_impl; tea. cbn. now intros ? ? [].
+        constructor; [|constructor]. apply ev2.
+      + rewrite ht. rewrite -remove_last_last //.
+      + eapply qapp in q as []; auto.
+        eapply qapp. split => //.
+      + eapply qapp in q as []. eapply qapp; auto. split => //.
+        eapply All_impl; tea; cbn; intuition auto.
+      + eapply All2_All_mix_left in X18; [|exact X16].
+        eapply All2_All_mix_right in X18; [|exact X19].
+        eapply All2_All_mix_left in X18; [|exact X17].
+        eapply All2_impl; tea; cbn.
+        intros x y [? [[] ?]].
+        red. intuition auto.
+      + rewrite isEtaExp_Constructor.
+        apply/andP. split. rewrite -(All2_length X18).
+        rewrite ht -remove_last_last //.
+        eapply All_forallb. eapply All_impl; tea. cbn; intuition auto.
+    * move=> /and4P [] etat0 etaargs etaa etat. 
+      split. eapply (X12 _ _ _ _ ev1); tea. 
+      1,4:(apply and_assum; [ih|hp' P'Q]).
+      intros. apply and_assum; [ih|hp' P'Q].
+      pose proof (decompose_app_inv da). clear cv.
+      apply PCUICNormal.negb_is_true => iscapp.
+      cbn in da. eapply (f_equal fst) in da. 
+      rewrite Prelim.fst_decompose_app_rec in da. cbn in *.
+      unfold isConstructApp in iscapp. rewrite da in iscapp. 
+      destruct t => //.
+      eapply (isEtaExp_mkApps_intro _ _ [a']) => //.
+      iheta q.
+      eapply All_tip.1. iheta q0.
+      eapply (isEtaExp_mkApps_intro _ _ [a']) => //. iheta q.
+      eapply All_tip.1. iheta q0.
+  - intros ise. split => //. eapply X14; tea.
+Qed.
+
+Lemma All_True {A} l : All (fun x : A => True) l.
+Proof.
+  induction l; intuition auto.
+Qed.
+
+#[export] Instance Qpreserves_True Σ : Qpreserves (fun _ _ => True) Σ.
+Proof.
+  split; intros; red; intros; try split; intuition auto.
+  { destruct t; try solve [constructor; auto; auto using All_True]. }
+  { destruct cst_body => //. }
+  all:apply All_True.
+Qed.
+
+Ltac destruct_nary_times :=
+  match goal with 
+  | [ H : _ × _ |- _ ] => destruct H
+  | [ H : [× _, _ & _] |- _ ] => destruct H 
+  | [ H : [× _, _, _ & _] |- _ ] => destruct H 
+  | [ H : [× _, _, _, _ & _] |- _ ] => destruct H 
+  end.
+
+Lemma eval_etaexp {fl : WcbvFlags} {Σ a a'} : 
+  isEtaExp_env Σ ->
+  wf_glob Σ ->
+  eval Σ a a' -> isEtaExp Σ a -> isEtaExp Σ a'.
+Proof.
+  intros etaΣ wfΣ ev eta.
+  generalize I. intros q. revert a a' q eta ev.
+  apply (eval_preserve_mkApps_ind fl Σ (fun _ x => isEtaExp Σ x) (fun _ _ => True)) => //.
+  all:intros; repeat destruct_nary_times.
+  all:intuition auto.
+  - rewrite isEtaExp_Constructor => //.
+    rewrite -(All2_length X0) H.
+    cbn; eapply All_forallb. eapply All2_All_right; tea.
+    cbn. intros x y []; auto.
+Qed.
